\subsection{Sums of powers}\label{subsec:sums-of-powers}
\begin{proposition}[Sums of odd powers]
    \label{prop:sum-of-odd-powers}
    \begin{align*}
        \sum_{n=1}^{p} n^{2m+1} = \sum_{n=1}^{p} \sum_{k=1}^{n} \sum_{r=0}^{m} \coeffA{m}{r} k^r (n-k)^r
    \end{align*}
\end{proposition}
In explicit view
\begin{align*}
    \sum_{n=1}^{p} n^{2m+1} = \sum_{r=0}^{m} \coeffA{m}{r} \bigg \{
    &[0^r + 1^r + 2^r + 3^r + \cdots (n-1)^r] \\
    + &[0^r + 2^r + 4^r + 6^r + \cdots (2n-4)^r] \\
    + &[0^r + 3^r + 6^r + 9^r + \cdots (3n-9)^r] \\
    + &[0^r + 4^r + 8^r + 12^r + \cdots (4n-16)^r] \\
    + &\cdots + (p^2 - p^2)^r
    \bigg \}
\end{align*}

\begin{proposition}[Sums of odd powers forward decomposition]
    \label{prop:sum-odd-power-decomposition-forward}
    For non-negative integers $m$ and $n$
    \begin{align*}
        \sum_{n=1}^{p} n^{2m+1} = \sum_{n=1}^{p} \sum_{k=1}^{n} \sum_{t=1}^{m+1} (-1)^{t+1} \binom{m+1}{t} T_{m} (n+t, k)
    \end{align*}
\end{proposition}

\begin{proposition}[Sum of odd powers backward decomposition]
    \label{prop:sum-odd-power-decomposition-backward}
    For non-negative integers $m$ and $n$
    \begin{align*}
        \sum_{n=1}^{p} n^{2m+1} = \sum_{n=1}^{p} \sum_{k=1}^{n} \sum_{t=1}^{m+1} (-1)^{t+1} \binom{m+1}{t} T_{m} (n-t, k)
    \end{align*}
\end{proposition}
