\begin{proposition}[Backward Recurrence for $T_m$]
    \label{prop:Tm-recurrence-backward}
    For non-negative integers $m$ and $n$
    \begin{align*}
        T_{m} (n, k) = \sum_{t=1}^{m+1} (-1)^{t+1} \binom{m+1}{t} T_{m} (n-t, k)
    \end{align*}
    \begin{proof}
        The polynomial $T_{m} (n,k)$ is a polynomial of degree $m$ in $n$.
        Thus, the backward difference with respect to $n$ is
        $\nabla^{m+1} T_{m} (n, k) = \sum_{t=0}^{m+1} (-1)^{t} \binom{m+1}{t} T_{m} (n-t, k) = 0$.
        By isolating $(-1)^{0} \binom{m+1}{0} T_{m} (n-0, k)$ yields
        $T_{m} (n, k) = (-1) \sum_{t=1}^{m+1} (-1)^{t} \binom{m+1}{t} T_{m} (n-t, k)$.
    \end{proof}
\end{proposition}

\begin{proposition}[Odd power backward decomposition]
    \label{prop:odd-power-decomposition-backward}
    For non-negative integers $m$ and $n$
    \begin{align*}
        n^{2m+1} = \sum_{k=1}^{n} \sum_{t=1}^{m+1} (-1)^{t+1} \binom{m+1}{t} T_{m} (n-t, k)
    \end{align*}
    \begin{proof}
        Direct consequence of~\eqref{theorem:odd-power-identity}
        and backward recurrence~\eqref{prop:Tm-recurrence-backward}.
    \end{proof}
\end{proposition}

\begin{proposition}[Odd power backward decomposition shifted]
    \label{prop:odd-power-decomposition-backward-shifted}
    For non-negative integers $m$ and $n$
    \begin{align*}
        n^{2m+1} = \sum_{k=0}^{n-1} \sum_{t=1}^{m+1} (-1)^{t+1} \binom{m+1}{t} T_{m} (n-t, k)
    \end{align*}
    \begin{proof}
        Direct consequence of~\eqref{theorem:odd-power-identity},
        backward recurrence~\eqref{prop:Tm-recurrence-backward}, and symmetry~\eqref{prop:Tm-symmetry}.
    \end{proof}
\end{proposition}

\begin{corollary}[Odd power backward decomposition $m-1$]
    \label{cor:odd-power-decomposition-m-1}
    \begin{align*}
        n^{2m-1} = \sum_{k=1}^{n} \sum_{t=1}^{m} (-1)^{t+1} \binom{m}{t} T_{m-1} (n-t, k)
    \end{align*}
    \begin{proof}
        By setting $m \rightarrow m-1$ to~\eqref{prop:odd-power-decomposition-backward}.
    \end{proof}
\end{corollary}

\begin{corollary}[Odd power backward decomposition $m-1$ shifted]
    \label{cor:odd-power-decomposition-m-1-shifted}
    \begin{align*}
        n^{2m-1} = \sum_{k=0}^{n-1} \sum_{t=1}^{m} (-1)^{t+1} \binom{m}{t} T_{m-1} (n-t, k)
    \end{align*}
    \begin{proof}
        By setting $m \rightarrow m-1$ to~\eqref{prop:odd-power-decomposition-backward-shifted}
        and by symmetry~\eqref{prop:Tm-symmetry}.
    \end{proof}
\end{corollary}
