\subsection{Binomial forms}\label{subsec:binomial-forms}

\begin{corollary}[Binomial form]
    \label{prop:odd-power-binomial-plus}
    For integers $n$ and $a$ such that $n-2a \geq 0$
    \begin{align*}
    (n+2a)^{2m+1} = \sum_{r=0}^{m} \sum_{k=-a+1}^{n+a} \coeffA{m}{r} (k-a)^r (n-k-a)^r
    \end{align*}
\end{corollary}

\begin{corollary}[Shifted binomial form]
    \label{prop:odd-power-binomial-plus-shifted}
    For integers $n$ and $a$ such that $n-2a \geq 0$
    \begin{align*}
    (n+2a)^{2m+1} = \sum_{r=0}^{m} \sum_{k=-a}^{n+a-1} \coeffA{m}{r} (k-a)^r (n-k-a)^r
    \end{align*}
\end{corollary}

\begin{corollary}[Centered binomial form]
    \label{cor:odd-power-binomial-centered}
    For integers $n$ and $a$ such that $n-2a \geq 0$
    \begin{align*}
    (n+a)^{2m+1} = \sum_{r=0}^{m} \sum_{k=-\frac{a}{2}+1}^{n+\frac{a}{2}} \coeffA{m}{r} \left( k-\frac{a}{2} \right)^r \left( n-k-\frac{a}{2} \right)^r
    \end{align*}
\end{corollary}

\begin{corollary}[Shifted centered binomial form]
    \label{cor:odd-power-binomial-centered-shifted}
    For integers $n$ and $a$ such that $n-2a \geq 0$
    \begin{align*}
    (n+a)^{2m+1} = \sum_{r=0}^{m} \sum_{k=-\frac{a}{2}}^{n+\frac{a}{2}-1} \coeffA{m}{r} \left( k-\frac{a}{2} \right)^r \left( n-k-\frac{a}{2} \right)^r
    \end{align*}
\end{corollary}

\begin{proposition}[Negated binomial form]
    \label{prop:odd-power-binomial}
    For integers $n$ and $a$ such that $n-2a \geq 0$
    \begin{align*}
    (n-2a)^{2m+1} = \sum_{r=0}^{m} \sum_{k=a+1}^{n-a} \coeffA{m}{r} (k-a)^r (n-k-a)^r
    \end{align*}
    \begin{proof}
        By observing the summation limits we can see that $k$ runs as $k=a+1,a+2,a+3,\ldots,a+n-a$, which
        implies that $(k-a)=1,2,3,\ldots, n$.
        By observing the term $(n-k-a)$ we see that $(n-k-a)=n-1,n-2,n-3,\ldots,0$.
        Thus, by reindexing the sum
        $(n-2a)^{2m+1} = \sum_{r=0}^{m} \sum_{k=1}^{n-2a} \coeffA{m}{r} (a+k-a)^r (n-(a+k)-a)^r$
        the statement~\eqref{prop:odd-power-binomial} is equivalent to~\eqref{theorem:odd-power-identity}
        with setting $n \rightarrow n-2a$.
    \end{proof}
\end{proposition}

\begin{corollary}[Shifted negated binomial form]
    \label{prop:odd-power-binomial-shifted}
    For integers $n$ and $a$ such that $n-2a \geq 0$
    \begin{align*}
    (n-2a)^{2m+1} = \sum_{r=0}^{m} \sum_{k=a}^{n-a-1} \coeffA{m}{r} (k-a)^r (n-k-a)^r
    \end{align*}
\end{corollary}

\begin{corollary}[Centered negated binomial form]
    \label{cor:odd-power-binomial-symmetric}
    For integers $n$ and $a$ such that $n-a \geq 0$
    \begin{align*}
    (n-a)^{2m+1} = \sum_{r=0}^{m} \sum_{k=\frac{a}{2}}^{n-\frac{a}{2}-1} \coeffA{m}{r} \left( k-\frac{a}{2} \right)^r \left(n-k-\frac{a}{2} \right)^r
    \end{align*}
\end{corollary}

\begin{corollary}[Shifted centered negated binomial form]
    \label{cor:odd-power-binomial-symmetric-shifted}
    For integers $n$ and $a$ such that $n-a \geq 0$
    \begin{align*}
    (n-a)^{2m+1} = \sum_{r=0}^{m} \sum_{k=\frac{a}{2}+1}^{n-\frac{a}{2}} \coeffA{m}{r} \left( k-\frac{a}{2} \right)^r \left(n-k-\frac{a}{2} \right)^r
    \end{align*}
\end{corollary}
