The paper~\cite{another_approach_to_get_derivative_of_odd_power} reveals a connection between
ordinary derivatives of odd power and partial derivatives of the function
\begin{align*}
    f_{y} (x, z) = \sum_{k=1}^{z} \sum_{r=0}^{y} \mathbf{A}_{y,r} k^r (x-k)^r
\end{align*}
Let be a fixed point $v\in \mathbb{N}$, then ordinary derivative $\frac{d}{dx} g_v (u)$ of the odd-power function $g_v(x) = x^{2v + 1}$
evaluate in point $u\in\mathbb{R}$ equals to partial derivative $(f_{v})^{'}_{x} (u, u)$ evaluate in point $(u, u)$ plus
partial derivative $(f_{v})^{'}_{z} (u, u)$ evaluate in point $(u, u)$
\begin{align*}
    \frac{d}{dx} g_v (u) = (f_{v})^{'}_{x} (u, u) + (f_{v})^{'}_{z} (u, u)
\end{align*}
